going to simplify neutral plan

LeanLambdaLibMathlib/LambdaLib/unification.lean
@@ -6,22 +6,57 @@ open QuotTerm
 in this file, i'll define the actual unification tactic
 -/
 
+theorem lam_body_rw {t1 t2 s1 s2} : (lam s1 t1 = lam s2 t2) = (t1 = t2) := by
+  apply propext
+  apply Iff.intro
+  · apply lam_body
+  · intros
+    subst_vars
+    exact alpha
+
+theorem const_inj_rw {c1 c2} : (const c1 = const c2) = (c1 = c2) := by
+  apply propext
+  apply Iff.intro
+  · apply const_inj
+  · intros; subst_vars; rfl
+
+theorem var_inj_rw {i1 i2} : (var i1 = var i2) = (i1 = i2) := by
+  apply propext
+  apply Iff.intro
+  · apply var_inj
+  · intros; subst_vars; rfl
+
+-- TODO: i think this and the next theorem will be redundant with the general neutral form cases?
+theorem var_not_const_rw {i c} : (var i = const c) = False := by
+  apply propext
+  apply Iff.intro
+  · apply var_not_const
+  · intros; contradiction
+
+theorem var_not_const_rw2 {i c} : (const c = var i) = False := by
+  rw (config := {occs := .pos [2]}) [propext (Iff.intro Eq.symm Eq.symm)]
+  apply var_not_const_rw
+
 macro "basic_lambda_solve" : tactic => `(tactic|
   repeat ( first
     | simp [lift_app, lift_lam, lift_var, lift_const, subst_app, subst_lam, subst_var,
-      liftLiftMulti, substLiftMulti, subst_const, liftMultiZero, beta] at *
+      liftLiftMulti, substLiftMulti, subst_const, liftMultiZero, beta,
+      lam_body_rw, const_inj_rw, var_inj_rw, var_not_const_rw, var_not_const_rw2] at *
     | subst_vars -- TODO: maybe only have this go on equations of type QTerm
   )
 )
 
 -- for example, we want this to work:
-
-theorem example1 (t1 t2 : QTerm)
+example (t1 t2 : QTerm)
   (H : < (λ x. x) {t1} > = <λ x. x>)
   : <{t1} {t2}> = t2 := by
-  --
   basic_lambda_solve
-  --
+
+example (H : <λ x. A> = <λ x. B>) : False := by
+  basic_lambda_solve
+
+example (H : <λ x. A> = <λ x. x>) : False := by
+  basic_lambda_solve
 
 /-
 there are two more cases i need unification to solve
@@ -46,14 +81,79 @@ inductive Lhs : Type where
 | var : Nat → Lhs
 | const : SynTerm.Constant → Lhs
 
-inductive NeutralWithArity : Lhs → Nat → QTerm → Prop where
-| const : ∀{c}, NeutralWithArity (Lhs.const c) 0 (const c)
-| var : ∀{n}, NeutralWithArity (Lhs.var n) 0 (var n)
-| app : ∀{lhs t a arg}, NeutralWithArity lhs a t → NeutralWithArity lhs (Nat.succ a) (app t arg)
+open SynTerm
 
+inductive NeutralWithArity : Lhs → Nat → Term → Prop where
+| const : ∀{c}, NeutralWithArity (Lhs.const c) 0 (Term.const c)
+| var : ∀{n}, NeutralWithArity (Lhs.var n) 0 (Term.var n)
+| app : ∀{lhs t a arg}, NeutralWithArity lhs a t
+  → NeutralWithArity lhs (Nat.succ a) (Term.app t arg)
+
+theorem stepNeutral {lhs a t1 t2} (step : (union Step StepEta) t1 t2)
+  (H : NeutralWithArity lhs a t1)
+  : NeutralWithArity lhs a t2 := by
+  cases step with
+  | r step => cases step with
+    | app1 step =>
+      cases H
+      constructor
+      apply (stepNeutral (union.r step))
+      assumption
+    | app2 _ =>
+      cases H
+      constructor
+      assumption
+    | beta =>
+      cases H with | app H => _
+      cases H
+    | lam _ => cases H
+  | s step => cases step with
+    | app1 step =>
+      cases H
+      constructor
+      apply (stepNeutral (union.s step))
+      assumption
+    | app2 _ =>
+      cases H
+      constructor
+      assumption
+    | _ => cases H
+
+theorem allstepNeutral {lhs a t1 t2} (step : AllStep t1 t2)
+  (H : NeutralWithArity lhs a t1)
+  : NeutralWithArity lhs a t2 := by
+  induction step with
+  | refl => assumption
+  | cons _ _ ih =>
+    apply ih
+    apply stepNeutral <;> assumption
+
+inductive QNeutralWithArity : Lhs → Nat → QTerm → Prop where
+| const : ∀{c}, QNeutralWithArity (Lhs.const c) 0 (const c)
+| var : ∀{n}, QNeutralWithArity (Lhs.var n) 0 (var n)
+| app : ∀{lhs t a arg}, QNeutralWithArity lhs a t → QNeutralWithArity lhs (Nat.succ a) (app t arg)
+
+theorem liftNeutralWithArity {lhs a t}
+  : NeutralWithArity lhs a t ↔ QNeutralWithArity lhs a (Quotient.mk _ t) := by
+  apply Iff.intro
+  ·
+    intro H
+    induction H with
+    | const =>
+      apply QNeutralWithArity.const
+      --
+      sorry
+    | var => sorry
+    | app _ _ => sorry
+    --
+    sorry
+  · sorry
+
+-- i need a theorem that says that 2 neutrals of different arities are unequal?
+-- or maybe prove this first on SynTerm.Terms?
 theorem nwa_inj {t} {lhs1 lhs2} {a1 a2}
-  (H1 : NeutralWithArity lhs1 a1 t)
-  (H2 : NeutralWithArity lhs2 a2 t)
+  (H1 : QNeutralWithArity lhs1 a1 t)
+  (H2 : QNeutralWithArity lhs2 a2 t)
   : a1 = a2 ∧ lhs1 = lhs2 := by
   induction H1 with -- try simp
   | @const c =>
@@ -73,8 +173,8 @@ theorem nwa_inj {t} {lhs1 lhs2} {a1 a2}
   --
 
 theorem neutral_unequal {t1 t2} {lhs1 lhs2} {a1 a2}
-  (H1 : NeutralWithArity lhs1 a1 t1)
-  (H2 : NeutralWithArity lhs2 a2 t2)
+  (H1 : QNeutralWithArity lhs1 a1 t1)
+  (H2 : QNeutralWithArity lhs2 a2 t2)
   (notsame : a1 ≠ a2 ∨ lhs1 ≠ lhs2)
   : t1 ≠ t2 := by
   --
